etch4/Etch/Stream3Deriving.lean
@@ -1,0 +1,107 @@
+import Etch.Stream3
+
+namespace Etch.Deriving.AttrOrder
+
+open Lean Elab Command Term Meta
+
+structure Options (α : Type u) where
+  (order : List α)
+  (localDecl : Bool := false)
+structure OptionsT where
+  (order : TSyntaxArray `term)
+  (localDecl : Bool)
+
+private def mkOptions (declName : Name) (stx : TSyntax ``Parser.Term.structInst) : TermElabM OptionsT := do
+  -- First do a type check just to be sure
+  let expectedType ← elabType (← `($(mkIdent ``Options) $(mkIdent declName)))
+  let expr ← StructInst.elabStructInst stx.raw (some expectedType)
+  let typ ← inferType expr
+  if expr.hasSorry || typ.hasSorry then
+    throwErrorAt stx "expression contains sorry"
+  trace[Elab.Deriving.attr_order_total] m!"elabStructInst returns {expr}; with type {typ}; expected {expectedType}"
+
+  -- Extract elements from syntax.
+  match stx.raw with
+  | `(Parser.Term.structInst| { $fields* })
+  | `(Parser.Term.structInst| { $fields* : $_ }) => do
+    let mut order := none
+    let mut localDecl := false
+    for field in fields.getElems do
+      match field with
+      | `(Parser.Term.structInstField| order := [$elems,*]) =>
+        order := some elems.getElems
+      | `(Parser.Term.structInstField| order := $_) =>
+        throwErrorAt field "incorrect argument format; must be order := [attr1, attr2, …]"
+      | `(Parser.Term.structInstField| localDecl := true) =>
+        localDecl := true
+      | `(Parser.Term.structInstField| localDecl := false) =>
+        localDecl := false
+      | `(Parser.Term.structInstField| localDecl := $v) =>
+        throwErrorAt v "incorrect argument format; must be true or false"
+      | _ => throwErrorAt field "unknown field"
+    match order with
+    | some elems => return { order := elems, localDecl : OptionsT }
+    | none => throwErrorAt stx "missing order field"
+  | _ => throwError "incorrect argument format; must be \{ order := [attr1, attr2, …] }"
+
+def mkOrder (declName : Name) (options : OptionsT) : CommandElabM Bool := do
+  let id := mkIdent declName
+  let prepareName (n : String) : MacroM Name :=
+    if options.localDecl then
+      -- Logic similar to `Lean.Elab.Command.mkInstanceName`
+      let rec getSuffix (m : Name) := match m with
+      | .anonymous => ""
+      | .str m "" => getSuffix m
+      | .str _ s => s
+      | .num m _ => getSuffix m
+      let n := if "inst".isPrefixOf n then
+                 n ++ (getSuffix declName.eraseMacroScopes).capitalize
+               else
+                 n
+      mkUnusedBaseName <| Name.mkSimple n
+    else
+      pure <| `_root_ ++ declName.str n
+  let ordID          := mkIdent <| (← liftMacroM <| prepareName "order")
+  let instOrdID      := mkIdent <| (← liftMacroM <| prepareName "instAttrOrder")
+  let ordHereID      := mkIdent <| (← liftMacroM <| prepareName "orderHere")
+  let instOrdTotalID := mkIdent <| (← liftMacroM <| prepareName "instAttrOrderTotal")
+
+  let ord ← `(command|
+    @[reducible] def $ordID : $(mkIdent ``Shape) $id :=
+      ⟨[$(options.order):term,*], by decide⟩)
+  let instOrd ← `(command|
+    @[reducible] instance $instOrdID:ident : $(mkIdent ``AttrOrder) $id :=
+      ⟨$ordID⟩)
+
+  let mut ordHereCases := #[]
+  for arg in options.order do
+    let alt ← `(Parser.Term.matchAltExpr| | $arg => $(mkIdent ``List.Find.here))
+    ordHereCases := ordHereCases.push alt
+  let ordHere ← `(command|
+    def $ordHereID : ∀ (i : $id), $(mkIdent ``List.Here) i ($(mkIdent ``Shape.val) ($(mkIdent ``AttrOrder.order) (self := $instOrdID)))
+    $ordHereCases:matchAlt*)
+
+  let instOrdTotal ← `(command|
+    instance $instOrdTotalID:ident : $(mkIdent ``AttrOrderTotal) $id :=
+      ⟨$ordHereID⟩)
+
+  let cmds := #[ord, instOrd, ordHere, instOrdTotal]
+  for cmd in cmds do
+    trace[Elab.Deriving.attr_order_total] cmd
+    elabCommand cmd
+  return true
+
+def mkOrderTotalInstanceHandler (declNames : Array Name) (args? : Option (TSyntax ``Parser.Term.structInst)) : CommandElabM Bool := do
+  if declNames.size != 1 then
+    return false -- mutually inductive types are not supported yet
+  else if let some args := args? then
+    let opts ← liftTermElabM <| mkOptions declNames[0]! args
+    mkOrder declNames[0]! opts
+  else
+    return false -- don't support automatically forming an order yet
+
+initialize
+  registerDerivingHandlerWithArgs ``AttrOrderTotal mkOrderTotalInstanceHandler
+  registerTraceClass `Elab.Deriving.attr_order_total
+
+end Etch.Deriving.AttrOrder
