etch4/Etch/Stream3Test.lean
@@ -1,0 +1,72 @@
+import Etch.Stream3
+import Etch.Stream3Deriving
+
+namespace Etch.Stream.Test
+
+inductive A
+| attr1 | attr2 | attr3
+deriving Repr, DecidableEq
+def A.toTag : A → String
+| attr1 => "attr1"
+| attr2 => "attr2"
+| attr3 => "attr3"
+instance A.represented : Represented A := ⟨A.toTag⟩
+open A (attr1 attr2 attr3)
+
+set_option trace.Elab.Deriving.attr_order_total true in
+deriving instance AttrOrderTotal with { order := [.attr1, .attr2, .attr3] } for A
+
+inductive A'
+| attr' : Fin 10 → A'
+deriving Repr, DecidableEq,
+AttrOrderTotal with { order := [.attr' 0, .attr' 1, .attr' 2, .attr' 3, .attr' 4,
+                                .attr' 5, .attr' 6, .attr' 7, .attr' 8, .attr' 9] }
+def A'.toTag : A' → String
+| attr' _ => "attr1"
+instance A'.represented : Represented A' := ⟨A'.toTag⟩
+open A' (attr')
+
+variable (i j k : A)
+#check (contract' i $ default [i, j])
+#check let a  : [j] →ₛ i := (contract' i (default [i, j])); a
+
+variable
+(s₁ : [attr1] →ₛ attr3)
+(s₂ : [attr2] →ₛ attr3)
+(srev : [attr2, attr1] →ₛ attr3)
+
+section v1
+def attr1Sublist : [attr1].SublistT A.order.val := .check' (by decide)
+def attr2Sublist : [attr2].SublistT A.order.val := .check' (by decide)
+
+#eval (mergeAttr attr1Sublist attr2Sublist).fst.val
+
+#check (s₂.mulMerge attr2Sublist attr1Sublist s₁) -- `: (mergeAttr attr2Sublist attr1Sublist).fst.val →ₛ attr3`
+#check (s₂.mulMerge attr2Sublist attr1Sublist s₁ : [attr1, attr2] →ₛ attr3)
+
+#check (s₂.mulMerge (.check' (by decide)) (.check' (by decide)) s₁) -- works
+-- Doesn't work ☹
+-- #check (s₂.mulMerge (.check' (by decide)) (.check' (by decide)) s₁ : [attr1, attr2] →ₛ attr3)
+
+end v1
+
+section v2
+#eval merge [attr1] [attr2]
+#check s₂.mul' s₁ -- `: [attr1, attr2] →ₛ attr3`
+
+-- #check srev.mul'' s₁
+-- failed to synthesize instance
+--   `AttrMerge' A.order.val [attr2, attr1] [attr1] ?m.287939`
+
+#eval decide (attr' 0 < attr' 1)
+#eval decide (attr' 9 < attr' 1)
+#eval merge [attr' 0, attr' 9] [attr' 8]
+variable
+(s₁ : [attr' 0, attr' 3, attr' 4, attr' 5, attr' 6, attr' 7, attr' 9] →ₛ attr' 4)
+(s₂ : [attr' 0, attr' 1, attr' 2, attr' 3, attr' 8] →ₛ attr' 4)
+-- Notice how fast this is.
+#check s₂.mul' s₁ -- `: [attr1, attr2] →ₛ attr3`
+
+end v2
+
+end Etch.Stream.Test
